finished completeness theorem

src/propositional_logic/completeness.lean
@@ -1,6 +1,10 @@
 import propositional_logic.semantics
 import propositional_logic.syntactics
 
+open formula
+
+section soundness
+
 variables {T : Theory} {φ : Formula}
 
 theorem soundness (h : syntactics.consequence T φ) : semantics.consequence T φ :=
@@ -18,3 +22,59 @@ begin
       exact semantics.consequence_P3 } },
   { exact semantics.consequence_modus_ponens ‹_› ‹_› }
 end
+
+end soundness
+
+section completeness
+
+local infix ` ⊢ `:50 := syntactics.consequence
+
+def model (T : Theory) : valuation :=
+λ var, T ⊢ Var var
+
+variables {T : Theory} {φ : Formula}
+
+open syntactics
+
+
+/- We are going to show that (syntactical) consistent and complete theories have a model. -/
+lemma model_models_iff_consequence (hcons : consistent T) (hcom : complete T) : 
+  T ⊢ φ ↔ eval (model T) φ :=
+begin
+  induction φ with v φ ψ hφ hψ φ hφ,
+  { refl },
+  { rw [semantics.eval_to, ← hφ, ← hψ],
+    exact consistent_complete.consequence_to_iff_consequence_of hcons hcom },
+  { rw semantics.eval_not,
+    rw consistent_complete.consequence_not_iff_not_consequence ‹_› ‹_›,
+    cc }
+end
+
+theorem model_models (hcons : consistent T) (hcom : complete T) :
+  model T ⊧ T :=
+begin
+  intro φ,
+  rw ← model_models_iff_consequence ‹_› ‹_›,
+  exact consequence_mem,
+end
+
+theorem completeness : semantics.consequence T φ → T ⊢ φ :=
+begin
+  contrapose!,
+  intro h,
+  have hTnφ := consistent_union_of_consistent_not_consequence h,
+  rcases hTnφ.exists_consistent_complete_extension with ⟨T', hs, hcons, hcom⟩,
+  apply (mt (semantics.consequence_trans ((by simp) : T ⊆ T ∪ {¬ᶠ φ}))),
+  apply (mt (semantics.consequence_trans hs)),
+  apply semantics.not_consequence_of_models_union_not (_ : model T' ⊧ T' ∪ {¬ᶠ φ}),
+  refine (semantics.subset_models _ (model_models ‹_› ‹_›)),
+  apply set.union_subset (rfl.subset : T' ⊆ T'),
+  rw set.union_subset_iff at hs,
+  exact hs.2
+end
+
+end completeness
+
+theorem semantics_iff_syntactics {T : Theory} {φ : Formula} : 
+  semantics.consequence T φ ↔ syntactics.consequence T φ :=
+⟨completeness, soundness⟩
